Makefile
@@ -1,0 +1,12 @@
+.PHONY: all build install clean
+
+all: build
+
+build:
+	dune build -p prod3
+
+install:
+	dune install -p prod3
+
+clean:
+	dune clean -p prod3
